Split examples.v out of wp.v. Define the tactic [wp].

theories/wp.v
@@ -1,54 +1,16 @@
 Require Import monads lang free eval spec handle.
 
+Global Opaque handle.
+
 (* Instantiate the generic [handle] with the [spec] monad. *)
 
 Definition wp η e φ :=
   run η e ∋ φ.
 
-(* An example. *)
-
-Definition ELet p e1 e2 :=
-  EMatch e1 (BCons (Branch p e2) BNil).
-
-Definition EUnit :=
-  ETuple ENil.
-
-Definition EConstant c :=
-  EData c EUnit.
-
-Definition EPair e1 e2 :=
-  ETuple (ECons e1 (ECons e2 ENil)).
-
-Definition PPair p1 p2 :=
-  PTuple (PCons p1 (PCons p2 PNil)).
-
-(* let x = (A (), B ()) in let (x1, x2) = x in x1 *)
-
-Definition example :=
-  ELet (PVar "x") (EPair (EConstant "A") (EConstant "B")) $
-  ELet (PPair (PVar "x1") (PVar "x2")) (EVar "x") $
-  EVar "x1".
-
-Eval cbv in eval EnvNil example.
-
-(* An example of reasoning about straight-line code. *)
-
-Goal wp EnvNil example (λ v, v = VData "A" (VTuple VNil)).
-Proof.
-  unfold wp, run. rewrite handle_fixed_point. cbv. reflexivity.
-Qed.
-
-(* let x = (z1, z2) in let (x1, x2) = x in x1 *)
-
-Definition example2 :=
-  ELet (PVar "x") (EPair (EVar "z1") (EVar "z2")) $
-  ELet (PPair (PVar "x1") (PVar "x2")) (EVar "x") $
-  EVar "x1".
-
-Goal
-  ∀ v1 v2,
-  let env := EnvCons "z1" v1 (EnvCons "z2" v2 EnvNil) in
-  wp env example2 (λ v, v = v1).
-Proof.
-  intros. unfold wp, run. rewrite handle_fixed_point. cbv. reflexivity.
-Qed.
+Ltac wp :=
+  (* Expose [handle (eval η e)] in the goal. *)
+  unfold wp, run;
+  (* Unfold the outer iteration in the loop. *)
+  rewrite handle_fixed_point;
+  (* Let Coq compute! *)
+  cbv.
