theories/examples.v
@@ -1,0 +1,50 @@
+Require Import monads lang free eval spec handle wp.
+
+(* TODO move elsewhere *)
+(* Syntax. *)
+
+Definition ELet p e1 e2 :=
+  EMatch e1 (BCons (Branch p e2) BNil).
+
+Definition EUnit :=
+  ETuple ENil.
+
+Definition EConstant c :=
+  EData c EUnit.
+
+Definition EPair e1 e2 :=
+  ETuple (ECons e1 (ECons e2 ENil)).
+
+Definition PPair p1 p2 :=
+  PTuple (PCons p1 (PCons p2 PNil)).
+
+(* let x = (A (), B ()) in let (x1, x2) = x in x1 *)
+
+Definition example :=
+  ELet (PVar "x") (EPair (EConstant "A") (EConstant "B")) $
+  ELet (PPair (PVar "x1") (PVar "x2")) (EVar "x") $
+  EVar "x1".
+
+Eval cbv in eval EnvNil example.
+
+(* An example of reasoning about straight-line code. *)
+
+Goal wp EnvNil example (λ v, v = VData "A" (VTuple VNil)).
+Proof.
+  wp. reflexivity.
+Qed.
+
+(* let x = (z1, z2) in let (x1, x2) = x in x1 *)
+
+Definition example2 :=
+  ELet (PVar "x") (EPair (EVar "z1") (EVar "z2")) $
+  ELet (PPair (PVar "x1") (PVar "x2")) (EVar "x") $
+  EVar "x1".
+
+Goal
+  ∀ v1 v2,
+  let env := EnvCons "z1" v1 (EnvCons "z2" v2 EnvNil) in
+  wp env example2 (λ v, v = v1).
+Proof.
+  intros. wp. reflexivity.
+Qed.
